extraction/theories/EArities.v
@@ -1,0 +1,233 @@
+
+From Coq Require Import Bool String List Program BinPos Compare_dec Omega.
+From MetaCoq.Template Require Import config utils monad_utils BasicAst AstUtils.
+From MetaCoq.PCUIC Require Import PCUICAst PCUICAstUtils PCUICInduction PCUICTyping PCUICMetaTheory PCUICWcbvEval PCUICLiftSubst PCUICInversion PCUICSR PCUICNormal PCUICSafeReduce PCUICSafeLemmata PCUICSafeChecker PCUICPrincipality PCUICGeneration.
+From MetaCoq.Extraction Require EAst ELiftSubst ETyping EWcbvEval Extract Prelim.
+From Equations Require Import Equations.
+Require Import String.
+Local Open Scope string_scope.
+Set Asymmetric Patterns.
+Import MonadNotation.
+
+
+
+(* Instance extraction_checker_flags : checker_flags := Build_checker_flags true false false. *)
+
+Definition is_prop_sort s :=
+  match Universe.level s with
+  | Some l => Level.is_prop l
+  | None => false
+  end.
+
+Require Import Extract.
+
+Definition Is_conv_to_Arity Σ Γ T := exists T', ∥red Σ Γ T T'∥ /\ isArity T'.
+
+Ltac terror := try match goal with [t : type_error |- typing_result _] => exact (TypeError t) end.
+           
+Lemma constructors_typed:
+  forall (Σ : list global_decl) (univs : constraints) (k : kername)
+    (m : mutual_inductive_body) (x : one_inductive_body) (t1 : term) 
+    (i0 : ident) (n0 : nat),
+    In (i0, t1, n0) (ind_ctors x) ->
+    on_inductive (fun Σ0 : global_context => lift_typing typing Σ0) (Σ, univs) k m ->
+    ∑ T, (Σ, univs);;; arities_context (ind_bodies m) |- t1 : T.
+Proof.
+  intros Σ univs k m x t1 i0 n0 H2 X0.
+Admitted.
+
+Lemma proj_typed:
+  forall (Σ : list global_decl) (univs : constraints) (k : kername)
+    (m : mutual_inductive_body) (x : one_inductive_body) (t1 : term) 
+    (i0 : ident) (H2 : In (i0, t1) (ind_projs x))
+    (X0 : on_inductive (fun Σ0 : global_context => lift_typing typing Σ0) (Σ, univs) k m),
+    ∑ T, (Σ, univs);;; [] |- t1 : T.
+Proof.
+  
+Admitted.
+
+Lemma context_conversion_red Σ Γ Γ' s t : wf Σ -> 
+  PCUICSR.conv_context Σ Γ Γ' -> red Σ Γ s t -> red Σ Γ' s t.
+Admitted.
+
+Lemma invert_cumul_arity_r (Σ : global_context) (Γ : context) (C : term) T :
+  wf Σ -> wf_local Σ Γ ->
+  isArity T ->
+  Σ;;; Γ |- C <= T -> Is_conv_to_Arity Σ Γ C.
+Proof.
+  intros wfΣ.
+  revert Γ C; induction T; cbn in *; intros Γ C wfΓ ? ?; try tauto.
+  - eapply invert_cumul_sort_r in X as (? & ? & ?).
+    exists (tSort x). split; sq; eauto.
+  - eapply invert_cumul_prod_r in X as (? & ? & ? & [] & ?); eauto.
+    eapply IHT2 in c0 as (? & ? & ?); eauto. sq.
+
+    exists (tProd x x0 x2). split; sq; cbn; eauto.
+    etransitivity. eauto.
+    eapply PCUICReduction.red_prod_r.
+
+    eapply context_conversion_red. eauto. 2:eauto.
+    econstructor. eapply conv_context_refl; eauto. 
+
+    econstructor. 2:eauto. 2:econstructor; eauto. 2:cbn. admit. admit.
+  -   admit.
+Admitted.
+
+Lemma invert_cumul_arity_l (Σ : global_context) (Γ : context) (C : term) T :
+  wf Σ -> wf_local Σ Γ ->
+  isArity C -> 
+  Σ;;; Γ |- C <= T -> Is_conv_to_Arity Σ Γ T.
+Proof.
+  intros wfΣ.
+  revert Γ T; induction C; cbn in *; intros Γ T wfΓ ? ?; try tauto.
+  - eapply invert_cumul_sort_l in X as (? & ? & ?).
+    exists (tSort x). split; sq; eauto.
+  - eapply invert_cumul_prod_l in X as (? & ? & ? & [] & ?); eauto.
+    eapply IHC2 in c0 as (? & ? & ?); eauto. sq.
+
+    exists (tProd x x0 x2). split; sq; cbn; eauto.
+    etransitivity. eauto.
+    eapply PCUICReduction.red_prod_r.
+
+    eapply context_conversion_red. eauto. 2:eauto.
+    econstructor. eapply conv_context_refl; eauto. 
+
+    econstructor. 2:eauto. 2:econstructor; eauto. 2:cbn. admit. admit.
+  - eapply invert_cumul_letin_l in X; eauto.
+Admitted.
+
+Lemma isWfArity_prod_inv:
+  forall (Σ : global_context) (Γ : context) (T : term) (x : name) (x0 x1 : term),
+    isWfArity typing Σ Γ (tProd x x0 x1) -> (∑ s : universe, Σ;;; Γ |- x0 : tSort s) ×   isWfArity typing Σ (Γ,, vass x x0) x1
+.
+Proof.
+  
+           
+           (* destruct X as (? & ? & ? & ?). cbn in e. *)
+           (* change (Γ ,, vass x x0) with (Γ ,,, [vass x x0]). unfold ",," in e. *)
+           (* revert e. *)
+           (* generalize ([vass x x0]). intros. *)
+           (* induction x1 in l, e |- *; cbn in *; try now inv e. *)
+           (* ++ inv e. repeat econstructor. cbn. eauto. *)
+           (* ++ eapply IHx1_2 in e as (? & ? & ? & ?). *)
+           (*    repeat econstructor. cbn. admit. admit. (* destArity stuff *) *)
+           (* ++ eapply IHx1_3 in e as (? & ? & ? & ?). *)
+           (*    repeat econstructor. cbn. admit. admit. (* destArity stuff *) *)
+  
+Admitted.
+
+Lemma arity_type_inv Σ Γ t T1 T2 : wf Σ -> wf_local Σ Γ ->
+  Σ ;;; Γ |- t : T1 -> isArity T1 -> Σ ;;; Γ |- t : T2 -> Is_conv_to_Arity Σ Γ T2.
+Proof.
+  intros wfΣ wfΓ. intros. eapply principal_typing in X as (? & ? & ? & ?). 2:eauto. 2:exact X0.
+
+
+  eapply invert_cumul_arity_r in c0 as (? & ? & ?); eauto. sq.
+  eapply PCUICCumulativity.red_cumul_inv in X.
+  eapply cumul_trans in c; eauto.  
+  
+  eapply invert_cumul_arity_l in c as (? & ? & ?); eauto. sq.
+  exists x1; split; sq; eauto.
+Qed.
+
+Lemma cumul_kind1 Σ Γ A B u :
+  wf Σ -> 
+  is_prop_sort u -> Σ ;;; Γ |- B : tSort u ->
+  Σ ;;; Γ |- A <= B -> Σ ;;; Γ |- A : tSort u.
+Proof.
+  
+Admitted.
+
+Lemma cumul_kind2 Σ Γ A B u :
+  wf Σ ->
+  is_prop_sort u -> Σ ;;; Γ |- A <= B ->
+  Σ ;;; Γ |- A : tSort u -> Σ ;;; Γ |- B : tSort u.
+Proof.
+Admitted.
+
+Lemma leq_universe_prop Σ u1 u2 :
+  wf Σ ->
+  leq_universe (snd Σ) u1 u2 ->
+  (is_prop_sort u1 \/ is_prop_sort u2) ->
+  (is_prop_sort u1 /\ is_prop_sort u2).
+Admitted.
+
+Lemma Is_type_app Σ Γ t L T :
+  wf Σ ->
+  Σ ;;; Γ |- mkApps t L : T ->
+  Is_Type_or_Proof Σ Γ t ->
+  Is_Type_or_Proof Σ Γ (mkApps t L).
+Proof.
+  intros. eapply type_mkApps_inv in X0 as (? & ? & [] & ?); try eassumption.
+  destruct X1 as (? & ? & [ | [u]]).
+  - eapply PCUICPrincipality.principal_typing in t2 as (? & ? & ? & ?). 2:eauto. 2:exact t0.
+    
+
+
+  (*   Lemma typing_spine_change : *)
+  (*     forall (Σ : global_context) (Γ : context) (t : term) (L : list term) (x1 : term), *)
+  (*       Σ;;; Γ |- t : x1 -> forall x x0 : term, Σ;;; Γ |- t : x -> typing_spine Σ Γ x L x0 -> typing_spine Σ Γ x1 L x0. *)
+  (*   Proof. *)
+  (*     intros Σ Γ t L x1 t2 x x0 t0 t1. *)
+  (*   Admitted. *)
+  (*   eapply typing_spine_change in t1. 3:eapply t0. 2:eapply t2. clear t0. *)
+  (*   revert t t2. *)
+  (*   dependent induction t1; intros. *)
+  (*   + cbn. exists ty. split; eauto. *)
+  (*   + cbn. eapply IHt1. admit. *)
+  (*     eauto. eauto. *)
+  (* - destruct p. *)
+Admitted.
+
+Lemma Is_type_lambda Σ Γ na T1 t :
+  wf Σ ->
+  Is_Type_or_Proof Σ Γ (tLambda na T1 t) ->
+  Is_Type_or_Proof Σ (vass na T1 :: Γ) t.
+Proof.
+  intros ? (T & ? & ?).
+  eapply inversion_Lambda in t0 as (? & ? & ? & ? & ?).
+  exists x0. split; eauto. destruct s as [ | (u & ? & ?)].
+  - left. admit.
+  - right. exists u. split; eauto.
+Admitted.
+
+Lemma Is_type_red Σ Γ t v:
+  wf Σ ->
+  red Σ Γ t v ->
+  Is_Type_or_Proof Σ Γ t ->
+  Is_Type_or_Proof Σ Γ v.
+Proof.
+  intros ? ? (T & ? & ?).
+  exists T. split.
+  - eapply subject_reduction; eauto.
+  - eauto.
+Qed.
+
+Lemma Is_type_eval Σ Γ t v:
+  wf Σ ->
+  eval Σ Γ t v ->
+  Is_Type_or_Proof Σ Γ t ->
+  Is_Type_or_Proof Σ Γ v.
+Proof.
+  intros; eapply Is_type_red. eauto.
+  eapply wcbeval_red; eauto. eauto.
+Qed.
+
+
+Lemma isArity_ind_type:
+  forall idecl : one_inductive_body, isArity (ind_type idecl).
+Proof.
+  intros idecl.
+Admitted.
+
+Lemma tConstruct_no_Type Σ ind c u x1 : wf Σ ->
+  Is_Type_or_Proof Σ [] (mkApps (tConstruct ind c u) x1) ->
+  Is_proof Σ [] (mkApps (tConstruct ind c u) x1).
+Proof.
+  intros wfΣ (? & ? & [ | (? & ? & ?)]).
+  - exfalso. eapply type_mkApps_inv in t as (? & ? & [] & ?); eauto.
+    eapply inversion_Construct in t as (? & ? & ? & ? & ? & ? & ?). destruct x5. destruct p. cbn in *.
+    admit.
+  - exists x, x0. eauto.
+Admitted.
+
