extraction/theories/Prelim.v
@@ -1,19 +1,25 @@
 (* Distributed under the terms of the MIT license.   *)
 
-From Coq Require Import Bool String List Program BinPos Compare_dec Omega Lia.
+From Coq Require Import Bool String List Program BinPos Compare_dec Omega.
 From MetaCoq.Template Require Import config utils monad_utils BasicAst AstUtils.
-From MetaCoq.PCUIC Require Import PCUICAst PCUICAstUtils PCUICInduction PCUICTyping PCUICWeakening PCUICSubstitution PCUICRetyping PCUICMetaTheory PCUICWcbvEval PCUICSR  PCUICClosed PCUICGeneration PCUICSafeChecker.
-From MetaCoq.Extraction Require Import EAst ELiftSubst ETyping EWcbvEval Extract.
-From Equations Require Import Equations.
+From MetaCoq.Extraction Require Import EAst ELiftSubst Extract.
+From MetaCoq.PCUIC Require Import PCUICTyping PCUICAst PCUICAstUtils PCUICInduction  PCUICWeakening PCUICSubstitution PCUICRetyping PCUICMetaTheory PCUICWcbvEval PCUICSR  PCUICClosed PCUICInversion PCUICGeneration PCUICSafeChecker.
+
+
 Require Import String.
-Local Open Scope list_scope.
+Local Open Scope string_scope.
 Set Asymmetric Patterns.
 Import MonadNotation.
 
+Module E := EAst.
+
+Require Import Lia.
 
 Existing Instance config.default_checker_flags.
 Module PA := PCUICAst.
 Module P := PCUICWcbvEval.
+
+Ltac inv H := inversion H; subst; clear H.
 
 Lemma nth_error_app_inv X (x : X) n l1 l2 :
   nth_error (l1 ++ l2) n = Some x -> (n < #|l1| /\ nth_error l1 n = Some x) \/ (n >= #|l1| /\ nth_error l2 (n - List.length l1) = Some x).
@@ -70,28 +76,24 @@ Qed.
 Lemma typing_spine_inv_app Σ x0 l x x1 :
   PCUICGeneration.typing_spine Σ [] x0 (l ++ [x]) x1 -> { '(x2, x3) : _ & (PCUICGeneration.typing_spine Σ [] x0 l x2) * (Σ ;;; [] |- x : x3)}%type.
 Proof.
-  intros. depind X. destruct l; inv H.
-  destruct l; invs H.
+  intros. depind X. destruct l; inv x.
+  destruct l; invs x.
   + eexists (_, _). split. econstructor; eauto.  eauto.
-  + specialize (IHX _ _ _ _ eq_refl) as ([] & []).
+  + specialize (IHX _ _ eq_refl) as ([] & []).
     eexists (_, _). split.  econstructor; eauto. eauto.
 Qed.
 
-Lemma typing_spine_inv:
-  forall (Σ : PCUICAst.global_context) (i : inductive) (pars arg : nat) (args : list PCUICAst.term) 
-    (a T : PCUICAst.term) (args' : list PCUICAst.term) (u' : universe_instance)
-    (H17 : nth_error args (pars + arg) = Some a) (x2 x3 : PCUICAst.term),
-    PCUICGeneration.typing_spine Σ [] x2 args x3 ->
-    Σ;;; [] |- x3 <= PCUICAst.mkApps (tInd (fst (fst (i, pars, arg))) u') args' -> {T & Σ;;; [] |- a : T}.
+Lemma typing_spine_inv args arg a Σ x2 x3 :
+  nth_error args (arg) = Some a ->
+  PCUICGeneration.typing_spine Σ [] x2 args x3 ->
+  {T & Σ;;; [] |- a : T}.
 Proof.
-  intros. simpl in *.
-  revert pars arg H17.
-  dependent induction X; intros pars arg H17.
+  intros. revert arg H.
+  dependent induction X; intros arg H17.
   - rewrite nth_error_nil in H17. congruence.
-  - destruct (pars + arg)%nat eqn:E.
+  - destruct (arg)%nat eqn:E.
     + cbn in H17. invs H17. eauto.
-    + cbn in H17. eapply IHX.
-      eauto. instantiate (2 := 0). eassumption.
+    + cbn in H17. eauto.
 Qed.
 
 Lemma typing_spine_cumul:
@@ -148,7 +150,7 @@ Qed.
 (** ** on mkApps *)
 
 Lemma emkApps_snoc a l b :
-  mkApps a (l ++ [b]) = tApp (mkApps a l) b.
+  E.mkApps a (l ++ [b]) = E.tApp (E.mkApps a l) b.
 Proof.
   revert a; induction l; cbn; congruence.
 Qed.
@@ -160,7 +162,7 @@ Proof.
 Qed.
 
 Lemma mkAppBox_repeat n a :
-  mkAppBox a n = mkApps a (repeat tBox n).
+  mkAppBox a n = E.mkApps a (repeat tBox n).
 Proof.
   revert a; induction n; cbn; firstorder congruence.
 Qed.
@@ -195,26 +197,29 @@ Qed.
 (* Admitted. *)
 
 
-Lemma decompose_app_rec_mkApps f l l' : EAstUtils.decompose_app_rec (mkApps f l) l' =
+Lemma decompose_app_rec_mkApps f l l' : EAstUtils.decompose_app_rec (E.mkApps f l) l' =
                                     EAstUtils.decompose_app_rec f (l ++ l').
 Proof.
   induction l in f, l' |- *; simpl; auto; rewrite IHl, ?app_nil_r; auto.
 Qed.
 
 Lemma decompose_app_mkApps f l :
-  isApp f = false -> EAstUtils.decompose_app (mkApps f l) = (f, l).
+  E.isApp f = false -> EAstUtils.decompose_app (E.mkApps f l) = (f, l).
 Proof.
   intros Hf. unfold EAstUtils.decompose_app. rewrite decompose_app_rec_mkApps. rewrite app_nil_r.
   destruct f; simpl in *; (discriminate || reflexivity).
 Qed.
 
-Lemma typing_spine_In:
-  forall (Σ : PCUICAst.global_context) (args : list PCUICAst.term) 
-    (x x0 : PCUICAst.term) (t0 : typing_spine Σ [] x args x0) 
-    (x1 : PCUICAst.term) (H : In x1 args), ∑ T1, Σ;;; [] |- x1 : T1.
-Proof.
-  intros Σ args x x0 t0 x1 H.
-Admitted.
+(* Lemma typing_spine_In: *)
+(*   forall (Σ : PCUICAst.global_context) (args : list PCUICAst.term)  *)
+(*     (x x0 : PCUICAst.term) (t0 : typing_spine Σ [] x args x0)  *)
+(*     (x1 : PCUICAst.term) (H : In x1 args), ∑ T1, Σ;;; [] |- x1 : T1. *)
+(* Proof. *)
+(*   intros. *)
+(*   eapply In_nth_error in H as []. *)
+  
+(*   intros Σ args x x0 t0 x1 H. *)
+(* Admitted. *)
 
 
 (* Lemma fix_subst_length mfix : *)
@@ -229,3 +234,302 @@ Admitted.
 (*   #|fix_subst mfix| = #|mfix|. *)
 (* Proof. *)
 (* Admitted. *)
+
+
+(** ** Prelim stuff, should move *)
+
+Lemma All2_right_triv {A B} {l : list A} {l' : list B} P :
+  All P l' -> #|l| = #|l'| -> All2 (fun _ b => P b) l l'.
+Proof.
+  induction 1 in l |- *; cbn; intros; destruct l; cbn in *; try omega; econstructor; eauto.
+Qed.
+
+Lemma All_repeat {A} {n P} x :
+  P x -> @All A P (repeat x n).
+Proof.
+  induction n; cbn; econstructor; eauto.
+Qed.
+
+Lemma Alli_impl {A} {P Q} (l : list A) {n} : Alli P n l -> (forall n x, P n x -> Q n x) -> Alli Q n l.
+Proof. induction 1; try constructor; intuition auto. Defined.
+
+
+Lemma All2_map_left {A B C} (P : A -> C -> Type) l l' (f : B -> A) :
+  All2 (fun x y => P (f x) y) l l' -> All2 P  (map f l) l'.
+Proof. intros. rewrite <- (map_id l'). eapply All2_map; eauto. Qed.
+
+Lemma All2_map_right {A B C} (P : A -> C -> Type) l l' (f : B -> C) :
+  All2 (fun x y => P x (f y)) l l' -> All2 P  l (map f l').
+Proof. intros. rewrite <- (map_id l). eapply All2_map; eauto. Qed.
+
+Lemma Forall2_Forall_right {A B} {P : A -> B -> Prop} {Q : B -> Prop} {l l'} :
+  Forall2 P l l' ->
+  (forall x y, P x y -> Q y) ->
+  Forall Q l'.
+Proof.
+  intros HF H. induction HF; constructor; eauto.
+Qed.
+
+Lemma All2_from_nth_error A B L1 L2 (P : A -> B -> Type) :
+  #|L1| = #|L2| ->
+                (forall n x1 x2, n < #|L1| -> nth_error L1 n = Some x1
+                                      -> nth_error L2 n = Some x2
+                                      -> P x1 x2) ->
+                All2 P L1 L2.
+Proof.
+  revert L2; induction L1; cbn; intros.
+  - destruct L2; inv H. econstructor.
+  - destruct L2; inv H. econstructor.
+    eapply (X 0); cbn; eauto. omega.
+    eapply IHL1. eauto.
+    intros. eapply (X (S n)); cbn; eauto. omega.
+Qed.
+
+Lemma All2_nth_error {A B} {P : A -> B -> Type} {l l'} n t t' :
+  All2 P l l' ->
+  nth_error l n = Some t ->
+  nth_error l' n = Some t' ->
+  P t t'.
+Proof.
+  intros Hall. revert n.
+  induction Hall; destruct n; simpl; try congruence.
+  eauto.
+Qed.
+
+Lemma All_In X (P : X -> Type) (l : list X) x : All P l -> In x l -> squash (P x).
+Proof.
+  induction 1; cbn; intros; destruct H.
+  - subst. econstructor. eauto.
+  - eauto.
+Qed.      
+
+Lemma nth_error_skipn A l m n (a : A) :
+  nth_error l (m + n) = Some a ->
+  nth_error (skipn m l) n = Some a.
+Proof.
+  induction m in n, l |- *.
+  - cbn. destruct l; firstorder.
+  - cbn. destruct l.
+    + inversion 1.
+    + eapply IHm.
+Qed.
+
+Lemma declared_inductive_inj {Σ mdecl mdecl' ind idecl idecl'} :
+  declared_inductive Σ mdecl' ind idecl' ->
+  declared_inductive Σ mdecl ind idecl ->
+  mdecl = mdecl' /\ idecl = idecl'.
+Proof.
+  intros [] []. unfold declared_minductive in *.
+  rewrite H in H1. inv H1. rewrite H2 in H0. inv H0. eauto.
+Qed.
+
+Lemma decompose_app_rec_inv2 {t l' f l} :
+  decompose_app_rec t l' = (f, l) ->
+  isApp f = false.
+Proof.
+  induction t in f, l', l |- *; try intros [= <- <-]; try reflexivity.
+  simpl. apply IHt1.
+Qed.
+
+Module Ee := EWcbvEval.
+
+Lemma value_app_inv L :
+  Ee.value (E.mkApps tBox L) ->
+  L = nil.
+Proof.
+  intros. depelim H.
+  - destruct L using rev_ind.
+    reflexivity.
+    rewrite emkApps_snoc in H. inv H.
+  - induction L using rev_ind.
+    + reflexivity.
+    + rewrite emkApps_snoc in x. inv x.
+  - induction L using rev_ind.
+    + reflexivity.
+    + rewrite emkApps_snoc in x. inv x.
+  - assert (EAst.isApp (EAst.tConstruct i k) = false) by reflexivity.
+    assert (EAst.isApp tBox = false) by reflexivity.
+    eapply decompose_app_mkApps in H0.
+    eapply decompose_app_mkApps in H1.
+    rewrite <- x in H1. rewrite H0 in H1.
+    inv H1.
+Qed.
+
+(** ** Prelim on eliminations  *)
+
+Lemma elim_restriction_works Σ Γ ind npar p c brs :
+  (Is_proof Σ Γ (tCase (ind, npar) p c brs) -> False) -> Informative Σ ind.
+Proof.
+Admitted.
+
+Lemma elim_restriction_works_proj Σ Γ  p c :
+  (Is_proof Σ Γ (tProj p c) -> False) -> Informative Σ (fst (fst p)).
+Proof.
+Admitted.
+
+Lemma length_of_btys {ind mdecl' idecl' args' u' p pty indctx pctx ps btys} :
+  types_of_case ind mdecl' idecl' (firstn (ind_npars mdecl') args') u' p pty = Some (indctx, pctx, ps, btys) ->
+  #|btys| = #|ind_ctors idecl'|.
+Proof.
+Admitted.
+
+Lemma tCase_length_branch_inv Σ Γ ind npar p n u args brs T m t :
+  wf Σ ->
+  Σ ;;; Γ |- tCase (ind, npar) p (mkApps (tConstruct ind n u) args) brs : T ->
+  nth_error brs n = Some (m, t) ->
+  (#|args| = npar + m)%nat.
+Admitted.
+
+(** ** Prelim on fixpoints *)
+
+Lemma fix_subst_nth mfix n :
+  n < #|mfix| ->
+  nth_error (fix_subst mfix) n = Some (tFix mfix (#|mfix| - n - 1)).
+Proof.
+  unfold fix_subst. generalize (#|mfix|).
+  intros m. revert n. induction m; cbn; intros.
+  - destruct n; inv H.
+  - destruct n.
+    + cbn. now rewrite <- minus_n_O.
+    + cbn. rewrite IHm. reflexivity. omega.
+Qed.
+
+Lemma efix_subst_nth mfix n :
+  n < #|mfix| ->
+  nth_error (ETyping.fix_subst mfix) n = Some (E.tFix mfix (#|mfix| - n - 1)).
+Proof.
+  unfold ETyping.fix_subst. generalize (#|mfix|).
+  intros m. revert n. induction m; cbn; intros.
+  - destruct n; inv H.
+  - destruct n.
+    + cbn. now rewrite <- minus_n_O.
+    + cbn. rewrite IHm. reflexivity. omega.
+Qed.
+
+Lemma subslet_fix_subst Σ mfix1 :
+  subslet Σ [] (PCUICTyping.fix_subst mfix1) (PCUICLiftSubst.fix_context mfix1).
+Proof.
+
+Admitted.
+
+(** ** Prelim on typing *)
+
+Lemma typing_subst_instance Σ Γ t T u :
+  wf Σ ->
+  Σ ;;; Γ |- t : T ->
+  Σ ;;; Γ |- PCUICUnivSubst.subst_instance_constr u t : PCUICUnivSubst.subst_instance_constr u T.
+Proof.
+Admitted.
+
+Require Import PCUIC.PCUICGeneration.
+
+Inductive red_decls Σ Γ Γ' : forall (x y : PCUICAst.context_decl), Type :=
+| conv_vass na na' T T' : isWfArity_or_Type Σ Γ' T' -> red Σ Γ T T' ->
+                      red_decls Σ Γ Γ' (PCUICAst.vass na T) (PCUICAst.vass na' T')
+
+| conv_vdef_type na na' b T T' : isWfArity_or_Type Σ Γ' T' -> red Σ Γ T T' ->
+                             red_decls Σ Γ Γ' (PCUICAst.vdef na b T) (PCUICAst.vdef na' b T')
+
+| conv_vdef_body na na' b b' T : Σ ;;; Γ' |- b' : T -> red Σ Γ b b' ->
+                                                  red_decls Σ Γ Γ' (PCUICAst.vdef na b T) (PCUICAst.vdef na' b' T).
+
+Notation red_context := (context_relation red_decls).
+
+Lemma env_prop_imp `{checker_flags} P1 P2 :
+  (forall Σ Γ t T, P1 Σ Γ t T -> P2 Σ Γ t T) ->
+  env_prop P1 -> env_prop P2.
+Proof.
+  (* intros. econstructor; *)
+  (*           specialize (X0 Σ wfΣ Γ wfΓ t T). *)
+  (* 2: now eapply X, X0. *)
+  (* destruct X0; eauto. cbv. destruct Σ. cbv in f. *)
+  (* clear - X f. *)
+  (* induction f. *)
+  (* - econstructor. eauto. *)
+  (* - econstructor. eapply IHf; eauto. *)
+  (*   eauto. destruct d. cbn in *. *)
+  (*   + destruct c0. cbv in *. *)
+  (*     destruct cst_body. eapply X. eauto. *)
+  (*     destruct o as []. exists x. *)
+  (*     eauto. *)
+  (*   + clear IHf. cbv in *. *)
+  (*     inv o. econstructor; eauto. *)
+  (*     * eapply Alli_impl. eassumption. intros.  *)
+  (*       inv X0. *)
+  (*       unshelve epose (_ : (on_constructors *)
+  (*                              (fun (Σ : list PCUICAst.global_decl × Universes.ConstraintSet.t_) (Γ : list PCUICAst.context_decl)  *)
+  (*                                 (t : PCUICAst.term) (T : option PCUICAst.term) => *)
+  (*                                 match T with *)
+  (*                                 | Some T0 => P2 Σ Γ t T0 *)
+  (*                                 | None => ∑ s : ∑ l : list (Universes.Level.t × bool), [] = l -> False, P2 Σ Γ t (PCUICAst.tSort s) *)
+  (*                                 end) (Σ, c) k m n x (PCUICAst.ind_ctors x)) *)
+  (*                      ). *)
+  (*       { *)
+  (*         clear - onConstructors X. eapply Alli_impl. eassumption. *)
+  (*         intros. inv X0. econstructor. inv X1. exists x1. eauto. *)
+  (*         destruct X2. exists x1. admit. *)
+  (*       }  *)
+        
+  (*       econstructor. eassumption. inv onArity. *)
+  (*       econstructor. eauto. intros. eapply onProjections in H. inv H. *)
+  (*       econstructor. all:eauto. *)
+  (*       eapply Alli_impl. eauto. intros. cbn in *. destruct X0. exists x1. eauto. *)
+  (*       instantiate (1 := o). *)
+  (*       unfold check_ind_sorts in *. *)
+  (*       destruct ?. intros. subst. destruct onConstructors. cbn in *. eauto. subst o. *)
+  (*       cbn. admit. admit. admit. *)
+  (*     * inv onParams. *)
+  (*       -- econstructor. *)
+  (*       -- econstructor. 2:{ destruct X1. eexists; eauto. } *)
+  (*          clear - X X0. induction X0. econstructor. *)
+  (*          econstructor. eauto. destruct t0. eexists; eauto. *)
+  (*          econstructor. eauto. eauto. *)
+  (*       -- unfold on_context. econstructor. *)
+  (*          2:{ eauto. } clear - X X0. induction X0. econstructor. *)
+  (*          econstructor. eauto. destruct t0. eexists; eauto. *)
+  (*          econstructor; eauto. *)
+Admitted.
+
+Lemma red_context_conversion :
+  env_prop
+    (fun (Σ : PCUICAst.global_context) (Γ : PCUICAst.context) (t T : PCUICAst.term) =>
+       forall Γ' : PCUICAst.context, red_context Σ Γ Γ' -> Σ;;; Γ' |- t : T).
+Proof.
+  eapply env_prop_imp. 2: eapply context_conversion.
+  intros. eapply X.
+  clear - X0.
+  Lemma red_conv_context:
+    forall (Σ : global_context) (Γ Γ' : context), red_context Σ Γ Γ' -> conv_context Σ Γ Γ'.
+  Proof.
+    intros Σ Γ Γ' X0.
+    induction X0.
+    - econstructor.
+    - econstructor. eauto. econstructor. inv p. eauto.
+      inv p. econstructor. now eapply PCUICCumulativity.red_cumul.
+      now eapply PCUICCumulativity.red_cumul_inv.
+    - econstructor. eauto. inv p.
+      econstructor. eauto. econstructor.
+      now eapply PCUICCumulativity.red_cumul.
+      now eapply PCUICCumulativity.red_cumul_inv.
+      econstructor. eauto.
+      econstructor.
+      now eapply PCUICCumulativity.red_cumul.
+      now eapply PCUICCumulativity.red_cumul_inv.
+  Qed.
+  now eapply red_conv_context.
+Qed.
+
+Lemma conv_context_app (Σ : global_context) (Γ1 Γ2 Γ1' : context) :
+  wf Σ ->
+  wf_local Σ (Γ1 ,,, Γ2) ->
+  conv_context Σ Γ1 Γ1' -> conv_context Σ (Γ1 ,,, Γ2) (Γ1' ,,, Γ2).
+Proof.
+  intros. induction Γ2.
+  - cbn; eauto.
+  - destruct a. destruct decl_body.
+    + cbn. econstructor. inv X0. eauto. econstructor. 2:eapply conv_refl.
+      inv X0. right. cbn in X3. destruct X3. exists x. eapply context_conversion; eauto.
+    + cbn. econstructor. inv X0. eauto. econstructor. 2:eapply conv_refl.
+      inv X0. right. cbn in X3. destruct X3. exists x. eapply context_conversion; eauto.
+Qed.
+
